AwsCryptographicMaterialProviders/dafny/AwsCryptographyKeyStoreAdmin/test/Mutations/TestEncryptionContextAddValue.dfy
@@ -47,14 +47,10 @@ module {:options "/functionSyntax:4" } TestMutationsEncryptionContextAddValue {
     var ddbClient :- expect DDB.DynamoDBClient();
     var kmsClient :- expect KMS.KMSClient();
 
-    var storage :- expect AdminFixtures.DefaultStorage();
+    var storage :- expect Fixtures.DefaultStorage();
+    var keyStore :- expect Fixtures.DefaultKeyStore();
     var underTest :- expect AdminFixtures.DefaultAdmin(ddbClient?:=Some(ddbClient));
     var strategy :- expect AdminFixtures.DefaultKeyManagerStrategy(kmsClient?:=Some(kmsClient));
-    var keyStore :- expect AdminFixtures.DefaultKeyStore();
-    // Recommend commenting the assume out while developing this method,
-    // and just ignore the modifies exeptions,
-    // and then re-enabling it once everything is safe
-    assume {:axiom} storage.Modifies == {} && underTest.Modifies == {} && keyStore.Modifies == {};
 
     var uuid :- expect UUID.GenerateUUID();
     var testId := happyCaseId + "-" + uuid;
@@ -63,7 +59,7 @@ module {:options "/functionSyntax:4" } TestMutationsEncryptionContextAddValue {
     var kodaBytes :- expect UTF8.Encode("Koda");
     var isADogBytes :- expect UTF8.Encode("is a dog.");
     var originalEC := map[kodaBytes := isADogBytes];
-    AdminFixtures.CreateHappyCaseId(id:=testId, versionCount:=0, customEC:=originalEC);
+    Fixtures.CreateHappyCaseId(id:=testId, versionCount:=0, customEC:=originalEC);
 
     print testLogPrefix + " Created the legit test items with 1 versions! testId: " + testId + "\n";
 
